Grass/Spec/Console.lean
@@ -1,0 +1,5 @@
+import Grass.Console.ContractCorrect
+
+namespace Grass
+export Specification (TextLine)
+end Grass
